src/Spec/Equiv.v
@@ -1,0 +1,189 @@
+Require Import ConcurProc.
+Require Import Relations.Relation_Operators.
+Require Import RelationClasses.
+Require Import Morphisms.
+Require Import Helpers.Helpers.
+
+Global Set Implicit Arguments.
+Global Generalizable All Variables.
+
+
+(** Matching traces *)
+
+Inductive traces_match {opLoT opMidT opHiT} :
+  forall (t1 : trace opLoT opMidT)
+         (t2 : trace opMidT opHiT), Prop :=
+
+| MatchLo : forall t1 t2 tid e,
+  traces_match t1 t2 ->
+  traces_match (TraceEvent tid (EvLow e) t1) t2
+
+| MatchInvokeMid : forall t1 t2 tid e,
+  traces_match t1 t2 ->
+  traces_match (TraceEvent tid (EvHigh e) t1)
+               (TraceEvent tid (EvLow e) t2)
+
+| MatchInvokeHi : forall t1 t2 tid e,
+  traces_match t1 t2 ->
+  traces_match t1 (TraceEvent tid (EvHigh e) t2)
+
+| MatchEmpty :
+  traces_match TraceEmpty TraceEmpty.
+
+Hint Constructors traces_match.
+
+
+Fixpoint trace_filter_hi `(t : trace opLoT opHiT) : trace opLoT opHiT :=
+  match t with
+  | TraceEmpty => TraceEmpty
+  | TraceEvent tid e t' =>
+    match e with
+    | EvLow _ => trace_filter_hi t'
+    | EvHigh _ => TraceEvent tid e (trace_filter_hi t')
+    end
+  end.
+
+Definition trace_match_hi {opLoT opHiT} (t1 t2 : trace opLoT opHiT) :=
+  trace_filter_hi t1 = trace_filter_hi t2.
+
+Instance trace_match_hi_preorder {opLoT opHiT} :
+  PreOrder `(@trace_match_hi opLoT opHiT).
+Proof.
+  split.
+  - firstorder.
+  - unfold trace_match_hi, Transitive; intros.
+    congruence.
+Qed.
+
+Lemma trace_match_hi_prepend : forall `(evs : list (event opT opHiT)) tr0 tr1 tid,
+  trace_match_hi tr0 tr1 ->
+  trace_match_hi (prepend tid evs tr0) (prepend tid evs tr1).
+Proof.
+  unfold trace_match_hi.
+  induction evs; simpl; intros; eauto.
+  destruct a; eauto.
+  erewrite IHevs; eauto.
+Qed.
+
+Hint Resolve trace_match_hi_prepend.
+
+
+Lemma trace_match_hi_drop_lo_l : forall opT opHiT e (tr1 tr2 : trace opT opHiT) tid,
+  trace_match_hi tr1 tr2 ->
+  trace_match_hi (TraceEvent tid (EvLow e) tr1) tr2.
+Proof.
+  unfold trace_match_hi; simpl; eauto.
+Qed.
+
+Lemma trace_match_hi_drop_lo_r : forall opLoT opHiT e (tr1 tr2 : trace opLoT opHiT) tid,
+  trace_match_hi tr1 tr2 ->
+  trace_match_hi tr1 (TraceEvent tid (EvLow e) tr2).
+Proof.
+  unfold trace_match_hi; simpl; eauto.
+Qed.
+
+Hint Resolve trace_match_hi_drop_lo_l.
+Hint Resolve trace_match_hi_drop_lo_r.
+
+
+(** Preserving traces for an entire threads_state *)
+
+Definition same_traces_s {opLo opHi State} op_step (s s' : State) (ts1 ts2 : @threads_state opLo opHi) :=
+  forall tr,
+    exec op_step s ts1 tr ->
+    exists tr', exec op_step s' ts2 tr' /\
+      trace_match_hi tr tr'.
+
+Definition same_traces {opLo opHi State} op_step (s : State) (ts1 ts2 : @threads_state opLo opHi) :=
+  same_traces_s op_step s s ts1 ts2.
+
+
+Instance same_traces_preorder {opT opHiT State op_step s} :
+  PreOrder (@same_traces opT opHiT State op_step s).
+Proof.
+  split.
+  - unfold Reflexive.
+    unfold same_traces, same_traces_s; intros.
+    eexists; intuition eauto.
+    reflexivity.
+  - unfold Transitive.
+    unfold same_traces, same_traces_s; intros.
+    eapply H in H1. deex.
+    eapply H0 in H1. deex.
+    eexists; intuition eauto.
+    etransitivity; eauto.
+Qed.
+
+
+(** A strong notion of execution equivalence, independent of semantics *)
+
+Definition exec_equiv_ts {opT opHiT} (ts1 ts2 : @threads_state opT opHiT) :=
+  forall State op_step (s : State) tr,
+    exec op_step s ts1 tr <->
+    exec op_step s ts2 tr.
+
+Definition exec_equiv_opt `(p1 : maybe_proc opT opHiT) p2 :=
+  forall (ts : threads_state) tid,
+    exec_equiv_ts (ts [[ tid := p1 ]]) (ts [[ tid := p2 ]]).
+
+Definition exec_equiv `(p1 : proc opT opHiT T) (p2 : proc _ _ T) :=
+  exec_equiv_opt (Proc p1) (Proc p2).
+
+Instance exec_equiv_ts_preorder {opLoT opHiT} :
+  PreOrder (@exec_equiv_ts opLoT opHiT).
+Proof.
+  split.
+  - firstorder.
+  - unfold Transitive, exec_equiv_ts; intros.
+    split; intros.
+    + apply H0. apply H. eauto.
+    + apply H. apply H0. eauto.
+Qed.
+
+
+(** Preserving traces for a single thread *)
+
+Definition trace_equiv_s `(s : State) s' tid `(op_step : OpSemantics opT State) `(p1 : proc opT opHiT T) (p2 : proc _ _ T) :=
+  forall ts,
+    same_traces_s op_step s s'
+      (ts [[ tid := Proc p1 ]])
+      (ts [[ tid := Proc p2 ]]).
+
+Definition trace_equiv {opT opHiT T} `(op_step : OpSemantics opT State) (p1 p2 : proc opT opHiT T) :=
+  forall ts s tid,
+    same_traces op_step s
+      (ts [[ tid := Proc p1 ]])
+      (ts [[ tid := Proc p2 ]]).
+
+
+Instance trace_equiv_preorder {opT opHiT T State op_step} :
+  PreOrder (@trace_equiv opT opHiT T State op_step).
+Proof.
+  split.
+  - unfold Reflexive; intros.
+    unfold trace_equiv; intros.
+    reflexivity.
+  - unfold Transitive; intros.
+    unfold trace_equiv; intros.
+    etransitivity; eauto.
+Qed.
+
+Instance trace_equiv_proper {opT opHiT T State op_step} :
+  Proper (Basics.flip (@trace_equiv opT opHiT T State op_step) ==>
+          @trace_equiv opT opHiT T State op_step ==>
+          Basics.impl) (@trace_equiv opT opHiT T State op_step).
+Proof.
+  intros p1 p2 H21 p3 p4 H34 H; subst.
+  unfold Basics.flip in *.
+  repeat (etransitivity; eauto).
+Qed.
+
+Instance trace_equiv_proper_flip {opT opHiT T State op_step} :
+  Proper (@trace_equiv opT opHiT T State op_step ==>
+          Basics.flip (@trace_equiv opT opHiT T State op_step) ==>
+          Basics.flip Basics.impl) (@trace_equiv opT opHiT T State op_step).
+Proof.
+  intros p1 p2 H21 p3 p4 H34 H; subst.
+  unfold Basics.flip in *.
+  repeat (etransitivity; eauto).
+Qed.
